Change the type [loc] to a type that is isomorphic but not equal to [Z].

theories/lang/locations.v
@@ -4,7 +4,20 @@ Local Open Scope Z_scope.
 
 (* A location is an integer. *)
 
-Definition loc := Z.
+(* We do not want Coq to think that [loc] and [Z] are the same type. Indeed,
+   the function [encode] does not work in the same way at memory locations
+   and at ordinary integers. For this reason, we use a record type. *)
+
+Record loc :=
+  Loc { address : Z }.
+
+(* These instances allow using locations as keys in sets and maps. *)
+
+Global Instance loc_eq_decision : EqDecision loc.
+Proof. solve_decision. Defined.
+
+Global Instance loc_countable : Countable loc.
+Proof. apply (inj_countable' address Loc). intros [?]. eauto. Defined.
 
 (* If needed, one could declare instances of the type classes [EqDecision],
    [Inhabited], [Countable], [Infinite] for the type [loc]. *)
@@ -13,13 +26,13 @@ Definition loc := Z.
    It is in the fact the least upper bound of the set [ls], except when [ls]
    is empty. *)
 
-Definition max_loc (ls : gset loc) : loc :=
-  set_fold Z.max 0 ls.
+Definition max_loc (ls : gset loc) : Z :=
+  set_fold (λ l accu, Z.max (address l) accu) 0 ls.
 
 Lemma le_max_loc :
-  ∀ ls l, l ∈ ls → l ≤ max_loc ls.
+  ∀ ls l, l ∈ ls → address l ≤ max_loc ls.
 Proof.
-  apply (set_fold_ind_L (λ r ls, ∀ l, l ∈ ls → l ≤ r)).
+  apply (set_fold_ind_L (λ r ls, ∀ l, l ∈ ls → address l ≤ r)).
   { set_solver. }
   { intros x X r _ IH l.
     rewrite elem_of_union, Z.max_le_iff.
@@ -30,13 +43,13 @@ Qed.
    finite set of locations [ls]. *)
 
 Definition fresh_loc (ls : gset loc) : loc :=
-  max_loc ls + 1.
+  {| address := max_loc ls + 1 |}.
 
 Lemma fresh_loc_fresh ls :
   fresh_loc ls ∉ ls.
 Proof.
   unfold fresh_loc.
   intro H.
-  specialize (le_max_loc _ _ H); clear H; intro H.
+  specialize (le_max_loc _ _ H); clear H; simpl; intro H.
   lia.
 Qed.
